hol/cake_sem/p4_arch_v1model_cakeScript.sml
@@ -15,7 +15,7 @@ val CONTROL_PLANE_API = 0;
 
 val _ = type_abbrev("v1model_sum_v_ext'", “:(core_v_ext', v1model_v_ext) sum”);
 
-Type v1model_ctrl' = “:(word64, (((e_list' -> bool) # num), word64 # e_list') alist) alist”;
+Type v1model_ctrl' = “:(word64, tbl) alist”;
 
 Type v1model_ascope' = “:(num # ((num, v1model_sum_v_ext') alist) # ((word64, v') alist) # v1model_ctrl')”;
 
@@ -223,6 +223,81 @@ Definition v1model_copyout_pbl'_def:
   | _ => NONE
 End
 
+
+Definition FOLDL_MATCH_alt'_def:
+ (FOLDL_MATCH_alt' w_l res acc [] = res) /\
+ (FOLDL_MATCH_alt' w_l (res_act, res_prio_opt:num option) acc (((s_l,prio),v)::t) =
+  if match_all_e_alt'' s_l w_l
+  then
+   (* TODO: Smallest priority wins (like for TDI) is hard-coded,
+    *       other than priority zero. *)
+   case res_prio_opt of
+   | SOME res_prio =>
+    let prio' = if (prio = 0) then acc else prio in
+    if (prio' < res_prio)
+    then
+     FOLDL_MATCH_alt' w_l (v, SOME prio') (acc+1) t
+    else FOLDL_MATCH_alt' w_l (res_act, res_prio_opt) (acc+1) t
+   | NONE => FOLDL_MATCH_alt' w_l (v, SOME prio) (acc+1) t
+  else FOLDL_MATCH_alt' w_l (res_act, res_prio_opt) (acc+1) t)
+End
+
+Definition FOLDL_MATCH'_def:
+ (FOLDL_MATCH' w_l res [] = res) /\
+ (FOLDL_MATCH' (w_l:word64 list) (res_act:word64 # e' list, res_prio_opt:num option) (((s_l,prio),v)::t) =
+  if match_all_e_alt'' s_l w_l
+  then
+   (* TODO: Largest priority wins (like for P4Runtime API) is hard-coded *)
+   case res_prio_opt of
+   | SOME res_prio =>
+    if prio > res_prio
+    then
+     FOLDL_MATCH' w_l (v, SOME prio) t
+    else FOLDL_MATCH' w_l (res_act, res_prio_opt) t
+   | NONE => FOLDL_MATCH' w_l (v, SOME prio) t
+  else FOLDL_MATCH' w_l (res_act, res_prio_opt) t)
+End
+
+val v1model_apply_table_f''_def =
+ if CONTROL_PLANE_API = 0
+ then xDefine "v1model_apply_table_f''"
+  ‘v1model_apply_table_f'' (x, e_l, mk_list:mk_list, (x', e_l'), (counter, ext_obj_map, v_map, ctrl):v1model_ascope') =
+    (* TODO: Note that this function could do other stuff here depending on table name.
+     *       Ideally, one could make a general, not hard-coded, solution for this *)
+    case ALOOKUP ctrl x of
+     | SOME table =>       
+      (case e_list_to_word64_list e_l of
+       | SOME w_l =>
+        (case table of
+           tbl_impl f => SOME $ f $ w_l
+         | tbl_regular tbl =>
+           if (MEM mk_lpm mk_list)
+           then
+            (* Largest priority wins (like for P4Runtime API - should be equivalent to TDI
+             * for tables that contain at most one LPM key, with others exact) *)
+            SOME (FST $ FOLDL_MATCH' w_l ((x', e_l'), NONE) tbl)
+           else
+            (* Smallest priority wins (like for TDI) *)
+            SOME (FST $ FOLDL_MATCH_alt' w_l ((x', e_l'), NONE) (1:num) tbl))
+       | NONE => NONE)
+     | NONE => NONE’
+ else xDefine "v1model_apply_table_f''"
+  ‘v1model_apply_table_f'' (x, e_l, mk_list:mk_list, (x', e_l'), (counter, ext_obj_map, v_map, ctrl):v1model_ascope') =
+    (* TODO: Note that this function could do other stuff here depending on table name.
+     *       Ideally, one could make a general, not hard-coded, solution for this *)
+    case ALOOKUP ctrl x of
+     | SOME table =>
+      (case e_list_to_word64_list e_l of
+       | SOME w_l =>
+        (case table of
+           tbl_impl f => SOME $ f $ w_l
+         | tbl_regular tbl =>
+          (* Largest priority wins *)
+          SOME (FST $ FOLDL_MATCH' w_l ((x', e_l'), NONE) table))
+       | NONE => NONE)
+     | NONE => NONE’;
+
+(* OLD:
 val v1model_apply_table_f'_def =
  if CONTROL_PLANE_API = 0
  then xDefine "v1model_apply_table_f'"
@@ -249,6 +324,7 @@ val v1model_apply_table_f'_def =
       (* Largest priority wins *)
       SOME (FST $ FOLDL_MATCH e_l ((x', e_l'), NONE) table)
      | NONE => NONE’;
+*)
 
 (** Implementations **)
 
