hol/cake_sem/p4_exec_sem_cakeProgScript.sml
@@ -183,7 +183,26 @@ val _ = translate bitv_eq_def;
 val _ = translate bitv_neq_def;
 val _ = translate get_bitv_binpred'_def;
 val _ = translate bitv_binpred'_def;
-val _ = translate p4_match_range'_def;
+
+Theorem word_msb_thm:
+ !w. word_msb (w:'a word) = BIT (dimindex (:'a) - 1) (w2n w)
+Proof
+ Cases \\ FULL_SIMP_TAC std_ss [word_msb_n2w,w2n_n2w]
+QED
+
+
+val _ = translate bitTheory.MOD_2EXP_def;
+val _ = translate bitTheory.DIV_2EXP_def;
+val _ = translate bitTheory.BITS_def;
+val _ = translate bitTheory.BIT_def;
+val _ = translate (word_msb_thm |> INST_TYPE [alpha|->``:64``] |> SIMP_RULE (srw_ss()) []);
+val _ = translate (word_mul_def |> INST_TYPE [alpha|->``:64``] |> SIMP_RULE (srw_ss()) []);
+val _ = translate (word_2comp_def |> INST_TYPE [alpha|->``:64``] |> SIMP_RULE (srw_ss()) [] |> SIMP_RULE std_ss [GSYM wordsTheory.WORD_NEG_MUL]);
+val _ = translate (nzcv_def |> INST_TYPE [alpha|->``:64``] |> SIMP_RULE (srw_ss()) []);
+val _ = translate (word_ge_def |> INST_TYPE [alpha|->``:64``]);
+val _ = translate (word_le_def |> INST_TYPE [alpha|->``:64``]);
+val _ = translate p4_match_range''_def;
+
 val _ = translate bitv_mul_def;
 val _ = translate bitv_div_def;
 val _ = translate bitv_mod_def;
@@ -226,12 +245,23 @@ val _ = translate p4Theory.binop2num_thm;
 val _ = translate p4Theory.binop_CASE;
 val _ = translate get_bitv_binop'_def;
 val _ = translate bitv_binop'_def;
-val _ = translate p4_match_mask'_def;
-val _ = translate match'_def;
-val _ = translate match_all'_def;
-val _ = translate match_all_first'_def;
+
+val _ = translate (EVAL “w2v (w:word64)” |> SIMP_RULE (srw_ss()) [word_bit_test,word_bit_def,word_bit]);
+val _ = translate (word_eq_def |> INST_TYPE [alpha|->``:64``] |> INST_TYPE [beta|->``:64``]);
+val _ = translate p4_match_mask''_def;
+val _ = translate match''_def;
+val _ = translate match_all''_def;
+val _ = translate match_all_first''_def;
+
+Theorem v2w_64_thm:
+ !v. v2w v = (n2w (v2n v)):word64
+Proof
+ FULL_SIMP_TAC std_ss [bitstringTheory.n2w_v2n]
+QED
+    
+val _ = translate v2w_64_thm;
+val _ = translate v_list_to_word64_list_def;
 val _ = translate match_all_first_def;
-val _ = translate v'_of_e'_def;
 val _ = translate e_exec_select'_def;
 
 (* Binops *)
